WIP PA 685

code/ecdsap256/Hacl.Impl.P256.PointAdd.fst
@@ -34,20 +34,26 @@ let point_eval c h p =
   felem_eval c h (gsub p (getCoordinateLenU64 c) (getCoordinateLenU64 c)) /\ 
   felem_eval c h (gsub p (size 2 *! getCoordinateLenU64 c) (getCoordinateLenU64 c)) 
 
-val getTempXYZ: #c: curve -> tempBuffer7: lbuffer uint64 (size 7 *! getCoordinateLenU64 c) -> 
+val getTempXYZ: #c: curve -> tempBuffer3: lbuffer uint64 (size 3 *! getCoordinateLenU64 c) -> 
   GTot (tuple3 (felem c) (felem c) (felem c))
-
-let getTempXYZ #c tempBuffer7 = 
+  
+let getTempXYZ #c tempBuffer3 = 
   let len = getCoordinateLenU64 c in 
-  let x3_out = gsub tempBuffer7 (size 0) len in 
-  let y3_out = gsub tempBuffer7 len len in 
-  let z3_out = gsub tempBuffer7 (size 2 *! len) len in 
+  let x3_out = gsub tempBuffer3 (size 0) len in 
+  let y3_out = gsub tempBuffer3 len len in 
+  let z3_out = gsub tempBuffer3 (size 2 *! len) len in 
   (x3_out, y3_out, z3_out)
 
 
 val getPointZ: #c: curve -> p: point c -> GTot (felem c)
 
 let getPointZ #c p = gsub p (size 2 *! getCoordinateLenU64 c) (getCoordinateLenU64 c)
+
+
+let felems_eval (c: curve) (h0: mem) (u1: felem c) (u2: felem c) (s1: felem c) (s2: felem c) (h: felem c) (uh: felem c) (r: felem c) (hCube: felem c) =  
+  felem_eval c h0 u1 /\ felem_eval c h0 u2 /\ felem_eval c h0 s1 /\
+  felem_eval c h0 s2 /\ felem_eval c h0 h /\ felem_eval c h0 uh /\ 
+  felem_eval c h0 r /\ felem_eval c h0 hCube
 
 
 #set-options "--z3rlimit 300" 
@@ -219,6 +225,28 @@ let copy_point_conditional #c x3_out y3_out z3_out p maskPoint =
   copy_conditional z3_out p_z mask
 
 
+let u1Invariant (#c: curve) (h : mem) (u1: felem c) (p: point c) (q: point c)  =  
+  let pxD= fromDomain_ #c (point_x_as_nat c h p) in 
+  let qzD = fromDomain_ #c (point_z_as_nat c h q) in 
+  felem_eval c h u1 /\ as_nat c h u1 == toDomain_ #c (qzD * qzD * pxD % getPrime c)
+
+
+let u2Invariant (#c: curve) (h: mem) (u2: felem c) (p: point c) (q: point c)  =  
+  let pzD = fromDomain_ #c (point_z_as_nat c h p) in 
+  let qxD  = fromDomain_ #c (point_x_as_nat c h q) in 
+  felem_eval c h u2 /\ as_nat c h u2 == toDomain_ #c (pzD * pzD * qxD % getPrime c)
+
+
+let s1Invariant (#c: curve) (h: mem) (s1: felem c) (p: point c) (q: point c)  = 
+  let pyD = fromDomain_ #c (point_y_as_nat c h p) in 
+  let qzD = fromDomain_ #c (point_z_as_nat c h q) in 
+  felem_eval c h s1 /\ as_nat c h s1 == toDomain_ #c (qzD * qzD * qzD * pyD % getPrime c)
+
+
+let s2Invariant (#c: curve) (h: mem) (s2: felem c) (p: point c) (q: point c)  = 
+  let pzD = fromDomain_ #c (point_z_as_nat c h p) in 
+  let qyD = fromDomain_ #c (point_y_as_nat c h q) in 
+  felem_eval c h s2 /\ as_nat c h s2 == toDomain_ #c (pzD * pzD * pzD * qyD % getPrime c)
 
 
 inline_for_extraction noextract 
@@ -231,24 +259,14 @@ val _move_from_jacobian_coordinates: #c: curve -> u1: felem c -> u2: felem c ->
     LowStar.Monotonic.Buffer.all_disjoint [loc tempBuffer4; loc p; loc q; loc u1; loc u2; loc s1; loc s2] /\ 
     point_eval c h p /\ point_eval c h q)
   (ensures fun h0 _ h1 ->  
-  
-    let prime = getPrime c in 
-    modifies (loc u1 |+| loc u2 |+| loc s1 |+| loc s2 |+| loc tempBuffer4) h0 h1 /\ 
-    felem_eval c h1 u1 /\ felem_eval c h1 u2 /\ felem_eval c h1 s1 /\ felem_eval c h1 s1 /\ (
-    let pX, pY, pZ = point_x_as_nat c h0 p, point_y_as_nat c h0 p, point_z_as_nat c h0 p in 
-    let qX, qY, qZ = point_x_as_nat c h0 q, point_y_as_nat c h0 q, point_z_as_nat c h0 q in 
-      
-    let pxD, pyD, pzD = fromDomain_ #c pX, fromDomain_ #c pY, fromDomain_ #c pZ in 
-    let qxD, qyD, qzD = fromDomain_ #c qX, fromDomain_ #c qY, fromDomain_ #c qZ in 
-
-    as_nat c h1 u1 == toDomain_ #c (qzD * qzD * pxD % prime) /\
-    as_nat c h1 u2 == toDomain_ #c (pzD * pzD * qxD % prime) /\
-    as_nat c h1 s1 == toDomain_ #c (qzD * qzD * qzD * pyD % prime) /\
-    as_nat c h1 s2 == toDomain_ #c (pzD * pzD * pzD * qyD % prime)
-    )
+    modifies (loc u1 |+| loc u2 |+| loc s1 |+| loc s2 |+| loc tempBuffer4) h0 h1 /\
+    u1Invariant #c h1 u1 p q /\
+    u2Invariant #c h1 u2 p q /\ 
+    s1Invariant #c h1 s1 p q /\
+    s2Invariant #c h1 s2 p q
   )
 
-
+ 
 let _move_from_jacobian_coordinates #c u1 u2 s1 s2 p q tempBuffer = 
   let h0 = ST.get() in 
 
@@ -289,49 +307,63 @@ let _move_from_jacobian_coordinates #c u1 u2 s1 s2 p q tempBuffer =
      lemma_mod_mul_distr_l (fromDomain_ #c (as_nat c h0 pZ) * fromDomain_ #c (as_nat c h0 pZ) * fromDomain_ #c (as_nat c h0 pZ)) (fromDomain_ #c (as_nat c h0 qY)) prime
 
 
+
 inline_for_extraction noextract 
 val move_from_jacobian_coordinates: #c: curve -> p: point c -> q: point c -> 
-  tempBuffer22: lbuffer uint64 (size 22 *! getCoordinateLenU64 c) -> 
+  tempBuffer12: lbuffer uint64 (size 12 *! getCoordinateLenU64 c) -> 
   Stack unit (requires fun h ->  
-    live h p /\ live h q /\ live h tempBuffer22 /\
-    LowStar.Monotonic.Buffer.all_disjoint [loc tempBuffer22; loc p; loc q] /\ 
+    live h p /\ live h q /\ live h tempBuffer12 /\
+    LowStar.Monotonic.Buffer.all_disjoint [loc tempBuffer12; loc p; loc q] /\ 
     point_eval c h p /\ point_eval c h q)
   (ensures fun h0 _ h1 ->  
-    let prime = getPrime c in 
     let len = getCoordinateLenU64 c in 
     
-    modifies (loc tempBuffer22) h0 h1 /\ (
-    let u1 = gsub tempBuffer22 (size 4 *! len) len in 
-    let u2 = gsub tempBuffer22 (size 5 *! len) len in 
-    let s1 = gsub tempBuffer22 (size 6 *! len) len in 
-    let s2 = gsub tempBuffer22 (size 7 *! len) len in 
-
-    felem_eval c h1 u1 /\ felem_eval c h1 u2 /\ felem_eval c h1 s1 /\ felem_eval c h1 s1 /\ (
-    let pX, pY, pZ = point_x_as_nat c h0 p, point_y_as_nat c h0 p, point_z_as_nat c h0 p in 
-    let qX, qY, qZ = point_x_as_nat c h0 q, point_y_as_nat c h0 q, point_z_as_nat c h0 q in 
-      
-    let pxD, pyD, pzD = fromDomain_ #c pX, fromDomain_ #c pY, fromDomain_ #c pZ in 
-    let qxD, qyD, qzD = fromDomain_ #c qX, fromDomain_ #c qY, fromDomain_ #c qZ in 
-
-    as_nat c h1 u1 == toDomain_ #c (qzD * qzD * pxD % prime) /\
-    as_nat c h1 u2 == toDomain_ #c (pzD * pzD * qxD % prime) /\
-    as_nat c h1 s1 == toDomain_ #c (qzD * qzD * qzD * pyD % prime) /\
-    as_nat c h1 s2 == toDomain_ #c (pzD * pzD * pzD * qyD % prime)
-    ) 
+    modifies (loc tempBuffer12) h0 h1 /\ (
+    let u1 = gsub tempBuffer12 (size 4 *! len) len in 
+    let u2 = gsub tempBuffer12 (size 5 *! len) len in 
+    let s1 = gsub tempBuffer12 (size 6 *! len) len in 
+    let s2 = gsub tempBuffer12 (size 7 *! len) len in 
+    
+    u1Invariant #c h1 u1 p q /\
+    u2Invariant #c h1 u2 p q /\ 
+    s1Invariant #c h1 s1 p q /\
+    s2Invariant #c h1 s2 p q)
   )
-)
 
-let move_from_jacobian_coordinates #c p q tempBuffer22 = 
+
+let move_from_jacobian_coordinates #c p q tempBuffer12 = 
   let len = getCoordinateLenU64 c in   
   
-  let tempBuffer4 = sub tempBuffer22 (size 0) (size 4 *! len) in 
+  let tempBuffer4 = sub tempBuffer12 (size 0) (size 4 *! len) in 
    
-  let u1 = sub tempBuffer22 (size 4 *! len) len in 
-  let u2 = sub tempBuffer22 (size 5 *! len) len in 
-  let s1 = sub tempBuffer22 (size 6 *! len) len in 
-  let s2 = sub tempBuffer22 (size 7 *! len) len in 
+  let u1 = sub tempBuffer12 (size 4 *! len) len in 
+  let u2 = sub tempBuffer12 (size 5 *! len) len in 
+  let s1 = sub tempBuffer12 (size 6 *! len) len in 
+  let s2 = sub tempBuffer12 (size 7 *! len) len in 
 
   _move_from_jacobian_coordinates #c u1 u2 s1 s2 p q tempBuffer4
+
+
+let hInvariant (#c: curve) (h0: mem) (h: felem c) (u1: felem c) (u2: felem c) = 
+  let u1D = fromDomain_ #c (as_nat c h0 u1) in 
+  let u2D = fromDomain_ #c (as_nat c h0 u2) in 
+  felem_eval c h0 h /\ as_nat c h0 h == toDomain_ #c ((u2D - u1D) % getPrime c)
+
+let rInvariant (#c: curve) (h0: mem) (r: felem c) (s1: felem c) (s2: felem c)  = 
+  let s1D = fromDomain_ #c (as_nat c h0 s1) in 
+  let s2D = fromDomain_ #c (as_nat c h0 s2) in 
+  felem_eval c h0 r /\ as_nat c h0 r == toDomain_ #c ((s2D - s1D) % getPrime c) 
+
+let uhInvariant (#c: curve) (h0: mem) (uh: felem c) (h: felem c) (u1: felem c) = 
+  let hD = fromDomain_ #c (as_nat c h0 h) in 
+  let u1D = fromDomain_ #c (as_nat c h0 u1) in 
+  felem_eval c h0 uh /\
+  as_nat c h0 uh == toDomain_ #c (hD * hD * u1D % getPrime c) 
+
+let hCubeInvariant (#c: curve) (h0 : mem) (hCube: felem c) (h: felem c) = 
+  let hD = fromDomain_ #c (as_nat c h0 h) in 
+  felem_eval c h0 hCube /\ as_nat c h0 hCube == toDomain_ #c (hD * hD * hD % getPrime c)
+
 
 
 inline_for_extraction noextract 
@@ -342,31 +374,15 @@ val _compute_common_params_point_add: #c: curve -> h: felem c -> r: felem c -> u
     (requires fun h0 -> 
       live h0 h /\ live h0 r /\ live h0 uh /\ live h0 hCube /\ live h0 u1 /\ 
       live h0 u2 /\ live h0 s1 /\ live h0 s2 /\ live h0 tempBuffer /\  
-      LowStar.Monotonic.Buffer.all_disjoint [loc u1; loc u2; loc s1; loc s2; loc h; loc r; loc uh; loc hCube; loc tempBuffer] /\ 
-      felem_eval c h0 u1 /\ 
-      felem_eval c h0 u2 /\
-      felem_eval c h0 s1 /\
-      felem_eval c h0 s2)
+      LowStar.Monotonic.Buffer.all_disjoint 
+	[loc u1; loc u2; loc s1; loc s2; loc h; loc r; loc uh; loc hCube; loc tempBuffer] /\ 
+      felem_eval c h0 u1 /\ felem_eval c h0 u2 /\  felem_eval c h0 s1 /\ felem_eval c h0 s2)
     (ensures fun h0 _ h1 -> 
-      modifies (loc h |+| loc r |+| loc uh |+| loc hCube |+| loc tempBuffer) h0 h1 /\ (
-      let prime = getPrime c in 
-      
-      felem_eval c h1 h /\ 
-      felem_eval c h1 r /\
-      felem_eval c h1 uh /\
-      felem_eval c h1 hCube /\ (
-      
-      let u1D = fromDomain_ #c (as_nat c h0 u1) in 
-      let u2D = fromDomain_ #c (as_nat c h0 u2) in 
-      let s1D = fromDomain_ #c (as_nat c h0 s1) in 
-      let s2D = fromDomain_ #c (as_nat c h0 s2) in 
-	
-      let hD = fromDomain_ #c (as_nat c h1 h) in 
-      
-      as_nat c h1 h == toDomain_ #c ((u2D - u1D) % prime) /\
-      as_nat c h1 r == toDomain_ #c ((s2D - s1D) % prime) /\
-      as_nat c h1 uh == toDomain_ #c (hD * hD * u1D % prime) /\
-      as_nat c h1 hCube == toDomain_ #c (hD * hD * hD % prime)))
+      modifies (loc h |+| loc r |+| loc uh |+| loc hCube |+| loc tempBuffer) h0 h1 /\ 
+      hInvariant #c h1 h u1 u2 /\
+      rInvariant #c h1 r s1 s2 /\
+      uhInvariant #c h1 uh h u1 /\
+      hCubeInvariant #c h1 hCube h
   )
 
 
@@ -389,56 +405,39 @@ let _compute_common_params_point_add #c h r uh hCube u1 u2 s1 s2 tempBuffer =
 
 
 val compute_common_params_point_add: #c: curve -> 
-  tempBuffer22: lbuffer uint64 (size 22 *! getCoordinateLenU64 c) -> 
-  Stack unit 
+  tempBuffer12: lbuffer uint64 (size 12 *! getCoordinateLenU64 c) -> Stack unit 
     (requires fun h0 ->
       let len = getCoordinateLenU64 c in 
     
-      let u1 = gsub tempBuffer22 (size 4 *! len) len in 
-      let u2 = gsub tempBuffer22 (size 5 *! len) len in 
-      let s1 = gsub tempBuffer22 (size 6 *! len) len in 
-      let s2 = gsub tempBuffer22 (size 7 *! len) len in 
+      let u1 = gsub tempBuffer12 (size 4 *! len) len in 
+      let u2 = gsub tempBuffer12 (size 5 *! len) len in 
+      let s1 = gsub tempBuffer12 (size 6 *! len) len in 
+      let s2 = gsub tempBuffer12 (size 7 *! len) len in 
       
-      live h0 tempBuffer22 /\  
-      felem_eval c h0 u1 /\ 
-      felem_eval c h0 u2 /\
-      felem_eval c h0 s1 /\
-      felem_eval c h0 s2
+      live h0 tempBuffer12 /\  
+      felem_eval c h0 u1 /\ felem_eval c h0 u2 /\ felem_eval c h0 s1 /\ felem_eval c h0 s2
     )
     (ensures fun h0 _ h1 -> 
-      modifies (loc tempBuffer22) h0 h1 /\ (
-      let prime = getPrime c in 
+      modifies (loc tempBuffer12) h0 h1 /\ (
       let len = getCoordinateLenU64 c in 
 
-      let u1 = gsub tempBuffer22 (size 4 *! len) len in 
-      let u2 = gsub tempBuffer22 (size 5 *! len) len in 
-      let s1 = gsub tempBuffer22 (size 6 *! len) len in 
-      let s2 = gsub tempBuffer22 (size 7 *! len) len in 
+      let u1 = gsub tempBuffer12 (size 4 *! len) len in 
+      let u2 = gsub tempBuffer12 (size 5 *! len) len in 
+      let s1 = gsub tempBuffer12 (size 6 *! len) len in 
+      let s2 = gsub tempBuffer12 (size 7 *! len) len in 
   
-      let h = gsub tempBuffer22 (size 8 *! len) len in 
-      let r = gsub tempBuffer22 (size 9 *! len) len in 
-      let uh = gsub tempBuffer22 (size 10 *! len) len in 
+      let h = gsub tempBuffer12 (size 8 *! len) len in 
+      let r = gsub tempBuffer12 (size 9 *! len) len in 
+      let uh = gsub tempBuffer12 (size 10 *! len) len in 
 
-      let hCube = gsub tempBuffer22 (size 11 *! len) len in 
+      let hCube = gsub tempBuffer12 (size 11 *! len) len in 
 
-      
-      felem_eval c h1 h /\ 
-      felem_eval c h1 r /\
-      felem_eval c h1 uh /\
-      felem_eval c h1 hCube /\ (
-      
-      let u1D = fromDomain_ #c (as_nat c h0 u1) in 
-      let u2D = fromDomain_ #c (as_nat c h0 u2) in 
-      let s1D = fromDomain_ #c (as_nat c h0 s1) in 
-      let s2D = fromDomain_ #c (as_nat c h0 s2) in 
-	
-      let hD = fromDomain_ #c (as_nat c h1 h) in 
-      
-      as_nat c h1 h == toDomain_ #c ((u2D - u1D) % prime) /\
-      as_nat c h1 r == toDomain_ #c ((s2D - s1D) % prime) /\
-      as_nat c h1 uh == toDomain_ #c (hD * hD * u1D % prime) /\
-      as_nat c h1 hCube == toDomain_ #c (hD * hD * hD % prime))) 
+      hInvariant #c h1 h u1 u2 /\
+      rInvariant #c h1 r s1 s2 /\
+      uhInvariant #c h1 uh h u1 /\
+      hCubeInvariant #c h1 hCube h
   )
+)
 
 
 let compute_common_params_point_add #c tempBuffer =
@@ -460,27 +459,33 @@ let compute_common_params_point_add #c tempBuffer =
   _compute_common_params_point_add #c h r uh hCube u1 u2 s1 s2 tempBuffer4
 
 
+let x3Invariant (#c: curve) (h0: mem) (x3: felem c) (r: felem c) (hCube: felem c) (uh: felem c) = 
+  let hCubeD = fromDomain_ #c (as_nat c h0 hCube) in 
+  let uhD = fromDomain_ #c (as_nat c h0 uh) in 
+  let rD = fromDomain_ #c (as_nat c h0 r) in 
+  felem_eval c h0 x3 /\ as_nat c h0 x3 == toDomain_ #c ((rD * rD - hCubeD - 2 * uhD) % getPrime c)
+
 
 inline_for_extraction noextract
 val _computeX3_point_add: #c : curve -> x3: felem c -> hCube: felem c -> uh: felem c -> 
-  r: felem c -> tempBuffer: lbuffer uint64 (size 4 *! getCoordinateLenU64 c) ->  
+  r: felem c -> tempBuffer: lbuffer uint64 (size 3 *! getCoordinateLenU64 c) ->  
   Stack unit 
   (requires fun h0 -> 
-    let prime = getPrime c in  
     live h0 x3 /\ live h0 hCube /\ live h0 uh /\ live h0 r /\ live h0 tempBuffer /\
-    disjoint hCube tempBuffer /\ disjoint uh tempBuffer /\ disjoint x3 tempBuffer /\
+    
+    disjoint hCube tempBuffer /\ 
+    disjoint uh tempBuffer /\ 
+    disjoint x3 tempBuffer /\ 
+    disjoint r tempBuffer /\ 
+    
+    disjoint x3 r /\
+    disjoint x3 hCube /\ disjoint x3 uh /\
+    
     felem_eval c h0 hCube /\ felem_eval c h0 uh /\ felem_eval c h0 r)
   (ensures fun h0 _ h1 -> 
-    let prime = getPrime c in 
     modifies (loc x3 |+| loc tempBuffer) h0 h1 /\ 
-    felem_eval c h1 x3 /\ 
-    (
-      let hCubeD = fromDomain_ #c (as_nat c h0 hCube) in 
-      let uhD = fromDomain_ #c (as_nat c h0 uh) in 
-      let rD = fromDomain_ #c (as_nat c h0 r) in 
-      as_nat c h1 x3 == toDomain_ #c ((rD * rD - hCubeD - 2 * uhD) % prime)
-    )  
-  )
+    x3Invariant #c h1 x3 r hCube uh)
+
 
 let _computeX3_point_add #c x3 hCube uh r tempBuffer = 
   let h0 = ST.get() in
@@ -491,83 +496,95 @@ let _computeX3_point_add #c x3 hCube uh r tempBuffer =
   let rH = sub tempBuffer len len in 
   let twoUh = sub tempBuffer (size 2 *! len) len in 
   montgomery_square_buffer r rSquare; 
-    let h1 = ST.get() in 
   felem_sub rSquare hCube rH;
-    let h2 = ST.get() in 
   multByTwo uh twoUh;
-    let h3 = ST.get() in 
   felem_sub rH twoUh x3; 
+    let h4 = ST.get() in 
 
   let prime = getPrime c in 
-  lemma_mod_add_distr (- fromDomain_ #c (as_nat c h1 hCube)) (fromDomain_ #c (as_nat c h0 r) * fromDomain_ #c (as_nat c h0 r)) prime;
-  lemma_mod_add_distr (- fromDomain_ #c (as_nat c h3 twoUh)) (fromDomain_ #c (as_nat c h0 r) * fromDomain_ #c (as_nat c h0 r) - fromDomain_ #c (as_nat c h1 hCube)) prime;
-  lemma_mod_sub_distr (fromDomain_ #c (as_nat c h0 r) * fromDomain_ #c (as_nat c h0 r) - fromDomain_ #c (as_nat c h1 hCube)) (2 * fromDomain_ #c (as_nat c h2 uh)) prime
+  let r = as_nat c h0 r in 
+
+  calc (==)
+  {
+    toDomain_ #c (((((fromDomain_ #c r * fromDomain_ #c r  % prime) - fromDomain_ #c (as_nat c h0 hCube)) % prime) - (2 * fromDomain_ #c (as_nat c h0 uh) % prime)) % prime);
+    (==) {lemma_mod_add_distr (- fromDomain_ #c (as_nat c h0 hCube)) (fromDomain_ #c r * fromDomain_ #c r) prime}
+    toDomain_ #c (((fromDomain_ #c r * fromDomain_ #c r - fromDomain_ #c (as_nat c h0 hCube)) % prime - (2 * fromDomain_ #c (as_nat c h0 uh) % prime)) % prime);
+    (==) {lemma_mod_sub_distr ((fromDomain_ #c r * fromDomain_ #c r - fromDomain_ #c (as_nat c h0 hCube)) % prime) (2 * fromDomain_ #c (as_nat c h0 uh)) prime}
+    toDomain_ #c (((fromDomain_ #c r * fromDomain_ #c r - fromDomain_ #c (as_nat c h0 hCube)) % prime - (2 * fromDomain_ #c (as_nat c h0 uh))) % prime);
+    (==) {lemma_mod_add_distr (- (2 * fromDomain_ #c (as_nat c h0 uh))) ((fromDomain_ #c r * fromDomain_ #c r - fromDomain_ #c (as_nat c h0 hCube))) prime}
+    toDomain_ #c ((fromDomain_ #c r * fromDomain_ #c r - fromDomain_ #c (as_nat c h0 hCube) - (2 * fromDomain_ #c (as_nat c h0 uh))) % prime);
+    (==) {_ by (canon())}
+    toDomain_ #c ((fromDomain_ #c r * fromDomain_ #c r - fromDomain_ #c (as_nat c h0 hCube) - 2 * fromDomain_ #c (as_nat c h0 uh)) % prime);
+  }
 
 
 val computex3_point_add: #c : curve -> hCube: felem c -> uh: felem c -> 
-  r: felem c -> tempBuffer7: lbuffer uint64 (size 7 *! getCoordinateLenU64 c) ->  
+  r: felem c -> tempBuffer5: lbuffer uint64 (size 5 *! getCoordinateLenU64 c) ->  
   Stack unit 
   (requires fun h0 -> 
-    live h0 hCube /\ live h0 uh /\ live h0 r /\ live h0 tempBuffer7 /\
-    disjoint hCube tempBuffer7 /\ disjoint uh tempBuffer7 /\
+    live h0 hCube /\ live h0 uh /\ live h0 r /\ live h0 tempBuffer5 /\
+    disjoint hCube tempBuffer5 /\ disjoint uh tempBuffer5 /\ disjoint r tempBuffer5 /\
     felem_eval c h0 hCube /\ felem_eval c h0 uh /\ felem_eval c h0 r)
   (ensures fun h0 _ h1 -> 
-    let prime = getPrime c in 
-    let x3 = gsub tempBuffer7 (size 0) (getCoordinateLenU64 c) in 
-    modifies (loc tempBuffer7) h0 h1 /\ felem_eval c h1 x3 /\ 
-    (
-      let hCubeD = fromDomain_ #c (as_nat c h0 hCube) in 
-      let uhD = fromDomain_ #c (as_nat c h0 uh) in 
-      let rD = fromDomain_ #c (as_nat c h0 r) in 
-      as_nat c h1 x3 == toDomain_ #c ((rD * rD - hCubeD - 2 * uhD) % prime)
-    )  
+    let x3 = gsub tempBuffer5 (size 0) (getCoordinateLenU64 c) in 
+    modifies (loc tempBuffer5) h0 h1 /\ 
+    x3Invariant #c h1 x3 r hCube uh
   )
 
 
-let computex3_point_add #c hCube uh r tempBuffer7 = 
-  let x3 = sub tempBuffer7 (size 0) (getCoordinateLenU64 c) in 
-  let tempBuffer4 = sub tempBuffer7 (size 3 *! getCoordinateLenU64 c) (size 4 *! getCoordinateLenU64 c) in 
-  _computeX3_point_add x3 hCube uh r tempBuffer4
-  
+let computex3_point_add #c hCube uh r tempBuffer4 = 
+  let len = getCoordinateLenU64 c in 
+  let x3 = sub tempBuffer4 (size 0) len in 
+  let tempBuffer3 = sub tempBuffer4 len (size 3 *! getCoordinateLenU64 c) in 
+  _computeX3_point_add x3 hCube uh r tempBuffer3
+
+
+let y3Invariant (#c: curve) (h0: mem) (y3: felem c) (s1: felem c) (hCube: felem c) (uh: felem c) (x3: felem c) (r: felem c) = 
+  let s1D = fromDomain_ #c (as_nat c h0 s1) in 
+  let hCubeD = fromDomain_ #c (as_nat c h0 hCube) in 
+  let uhD = fromDomain_ #c (as_nat c h0 uh) in 
+  let x3D = fromDomain_ #c (as_nat c h0 x3) in 
+  let rD = fromDomain_ #c (as_nat c h0 r) in 
+  felem_eval c h0 y3 /\ 
+  as_nat c h0 y3 = toDomain_ #c (((uhD - x3D) * rD - s1D * hCubeD) % getPrime c)
+
 
 inline_for_extraction noextract 
 val _computeY3_point_add: #c: curve -> y3: felem c -> s1: felem c -> 
   hCube: felem c -> uh: felem c -> x3_out: felem c -> r: felem c -> 
-  tempBuffer: lbuffer uint64 (size 4 *! getCoordinateLenU64 c) -> 
+  tempBuffer3: lbuffer uint64 (size 3 *! getCoordinateLenU64 c) -> 
   Stack unit 
     (requires fun h -> 
       let prime = getPrime c in 
       live h y3 /\ live h s1 /\ live h hCube /\ live h uh /\ live h x3_out /\ 
-      live h r /\ live h tempBuffer /\ 
-      disjoint uh tempBuffer /\
-      disjoint x3_out tempBuffer /\
-      disjoint y3 tempBuffer /\
-      disjoint r tempBuffer /\
+      live h r /\ live h tempBuffer3 /\ 
+      
+      disjoint uh tempBuffer3 /\
+      disjoint x3_out tempBuffer3 /\
+      disjoint y3 tempBuffer3 /\
+      disjoint r tempBuffer3 /\
+      disjoint s1 tempBuffer3 /\
+      disjoint hCube tempBuffer3 /\ 
+
+      disjoint y3 s1 /\ disjoint y3 hCube /\ disjoint y3 uh /\ disjoint y3 x3_out /\ disjoint y3 r /\
+      
       felem_eval c h s1 /\ 
       felem_eval c h hCube /\
       felem_eval c h uh/\ 
       felem_eval c h x3_out /\ 
       felem_eval c h r)
-    (ensures fun h0 _ h1 -> 
-      let prime = getPrime c in 
-      modifies (loc y3 |+| loc tempBuffer) h0 h1 /\ felem_eval c h1 y3 /\ 
-      (
-	let s1D = fromDomain_ #c (as_nat c h0 s1) in 
-	let hCubeD = fromDomain_ #c (as_nat c h0 hCube) in 
-	let uhD = fromDomain_ #c (as_nat c h0 uh) in 
-	let x3D = fromDomain_ #c (as_nat c h0 x3_out) in 
-	let rD = fromDomain_ #c (as_nat c h0 r) in 
-	as_nat c h1 y3 = toDomain_ #c (((uhD - x3D) * rD - s1D * hCubeD) % prime))
-      )
+    (ensures fun h0 _ h1 ->
+      modifies (loc y3 |+| loc tempBuffer3) h0 h1 /\ 
+      y3Invariant #c h1 y3 s1 hCube uh x3_out r)
+      
 
-
-let _computeY3_point_add #c y3 s1 hCube uh x3 r tempBuffer = 
+let _computeY3_point_add #c y3 s1 hCube uh x3 r tempBuffer3 = 
   let h0 = ST.get() in
   
   let len = getCoordinateLenU64 c in 
-  let s1hCube = sub tempBuffer (size 0) len in 
-  let u1hx3 = sub tempBuffer len len in 
-  let ru1hx3 = sub tempBuffer (size 2 *! len) len in 
+  let s1hCube = sub tempBuffer3 (size 0) len in 
+  let u1hx3 = sub tempBuffer3 len len in 
+  let ru1hx3 = sub tempBuffer3 (size 2 *! len) len in 
 
   montgomery_multiplication_buffer s1 hCube s1hCube;
   felem_sub uh x3 u1hx3; 
@@ -575,23 +592,46 @@ let _computeY3_point_add #c y3 s1 hCube uh x3 r tempBuffer =
   felem_sub #c ru1hx3 s1hCube y3;
 
   let h3 = ST.get() in 
-  let prime = getPrime c in
-    lemma_mod_mul_distr_l (fromDomain_ #c (as_nat c h0 uh) - fromDomain_ #c (as_nat c h0 x3)) (fromDomain_ #c (as_nat c h0 r)) prime;
 
-    lemma_mod_add_distr (- (fromDomain_ #c (as_nat c h3 s1hCube)))  ((fromDomain_ #c (as_nat c h0 uh) - fromDomain_ #c (as_nat c h0 x3)) * fromDomain_ #c (as_nat c h0 r)) prime;
-    lemma_mod_sub_distr ((fromDomain_ #c (as_nat c h0 uh) - fromDomain_ #c (as_nat c h0 x3)) * fromDomain_ #c (as_nat c h0 r)) (fromDomain_ #c (as_nat c h0 s1) * fromDomain_ #c (as_nat c h0 hCube)) prime
+
+  let prime = getPrime c in
+
+  let s1D = fromDomain_ #c (as_nat c h0 s1) in 
+  let hCubeD = fromDomain_ #c (as_nat c h0 hCube) in 
+  let uhD = fromDomain_ #c (as_nat c h0 uh) in 
+  let x3D = fromDomain_ #c (as_nat c h0 x3) in 
+  let rD = fromDomain_ #c (as_nat c h0 r) in 
+
+  calc (==)
+  {
+    toDomain_ #c (((uhD - x3D) % prime * rD % prime  - (s1D * hCubeD % prime)) % getPrime c);
+    (==) {lemma_mod_mul_distr_l (uhD - x3D) rD prime}
+    toDomain_ #c (((uhD - x3D) * rD % prime  - (s1D * hCubeD % prime)) % getPrime c);
+    (==) {_ by (canon())}
+    toDomain_ #c (((uhD - x3D) * rD % prime  - s1D * hCubeD % prime) % getPrime c);
+    (==) {lemma_mod_sub_distr ((uhD - x3D) * rD % prime) (s1D * hCubeD) prime}
+    toDomain_ #c (((uhD - x3D) * rD % prime - s1D * hCubeD) % getPrime c);
+    (==) {lemma_mod_add_distr (-s1D * hCubeD) ((uhD - x3D) * rD) prime}
+    toDomain_ #c (((uhD - x3D) * rD - s1D * hCubeD) % getPrime c);
+  }
 
 
 val computeY3_point_add: #c: curve -> s1: felem c -> hCube: felem c -> uh: felem c -> r: felem c -> 
-  tempBuffer7: lbuffer uint64 (size 7 *! getCoordinateLenU64 c) -> 
+  tempBuffer5: lbuffer uint64 (size 5 *! getCoordinateLenU64 c) -> 
   Stack unit 
     (requires fun h -> 
       let prime = getPrime c in 
-      let x3_out = gsub tempBuffer7 (size 0) (getCoordinateLenU64 c) in 
-      live h s1 /\ live h hCube /\ live h uh /\ live h r /\ live h tempBuffer7 /\ 
+      let x3_out = gsub tempBuffer5 (size 0) (getCoordinateLenU64 c) in 
+      live h s1 /\ live h hCube /\ live h uh /\ live h r /\ live h tempBuffer5 /\ 
       
-      disjoint uh tempBuffer7 /\
-      disjoint r tempBuffer7 /\
+      disjoint uh tempBuffer5 /\
+      disjoint x3_out tempBuffer5 /\
+      disjoint r tempBuffer5 /\
+      disjoint s1 tempBuffer5 /\
+      disjoint hCube tempBuffer5 /\ 
+
+      disjoint tempBuffer5 s1 /\ disjoint tempBuffer5 hCube /\ disjoint tempBuffer5 uh /\ 
+      disjoint tempBuffer5 x3_out /\ disjoint tempBuffer5 r /\
       
       felem_eval c h s1 /\ 
       felem_eval c h hCube /\
@@ -599,46 +639,40 @@ val computeY3_point_add: #c: curve -> s1: felem c -> hCube: felem c -> uh: felem
       felem_eval c h x3_out /\ 
       felem_eval c h r)
     (ensures fun h0 _ h1 -> 
-      let prime = getPrime c in 
-      let x3_out = gsub tempBuffer7 (size 0) (getCoordinateLenU64 c) in 
-      let y3_out = gsub tempBuffer7 (getCoordinateLenU64 c) (getCoordinateLenU64 c) in 
-      modifies (loc tempBuffer7) h0 h1 /\ felem_eval c h1 y3_out /\ 
+      let x3_out = gsub tempBuffer5 (size 0) (getCoordinateLenU64 c) in 
+      let y3_out = gsub tempBuffer5 (getCoordinateLenU64 c) (getCoordinateLenU64 c) in 
+      modifies (loc tempBuffer5) h0 h1 /\
       as_nat c h0 x3_out == as_nat c h1 x3_out /\
-      (
-	let s1D = fromDomain_ #c (as_nat c h0 s1) in 
-	let hCubeD = fromDomain_ #c (as_nat c h0 hCube) in 
-	let uhD = fromDomain_ #c (as_nat c h0 uh) in 
-	let x3D = fromDomain_ #c (as_nat c h0 x3_out) in 
-	let rD = fromDomain_ #c (as_nat c h0 r) in 
-	as_nat c h1 y3_out = toDomain_ #c (((uhD - x3D) * rD - s1D * hCubeD) % prime))
-      )
+      y3Invariant #c h1 y3_out s1 hCube uh x3_out r)
+ 
 
 
-let computeY3_point_add #c s1 hCube uh r tempBuffer7 = 
-  let x3 = sub tempBuffer7 (size 0) (getCoordinateLenU64 c) in 
-  let y3 = sub tempBuffer7 (getCoordinateLenU64 c) (getCoordinateLenU64 c) in 
-  let tempBuffer4 = sub tempBuffer7 (size 3 *! getCoordinateLenU64 c) (size 4 *! getCoordinateLenU64 c) in 
-  _computeY3_point_add #c y3 s1 hCube uh x3 r tempBuffer4
+let computeY3_point_add #c s1 hCube uh r tempBuffer5 = 
+  let x3 = sub tempBuffer5 (size 0) (getCoordinateLenU64 c) in 
+  let y3 = sub tempBuffer5 (getCoordinateLenU64 c) (getCoordinateLenU64 c) in 
+  let tempBuffer3 = sub tempBuffer5 (size 2 *! getCoordinateLenU64 c) (size 3 *! getCoordinateLenU64 c) in 
+  _computeY3_point_add #c y3 s1 hCube uh x3 r tempBuffer3
+
+
+let z3Invariant (#c: curve) (h0: mem) (z3: felem c) (z1: felem c) (z2: felem c) (h: felem c) = 
+  let z1D = fromDomain_ #c (as_nat c h0 z1) in 
+  let z2D = fromDomain_ #c (as_nat c h0 z2) in 
+  let hD = fromDomain_ #c (as_nat c h0 h) in 
+  felem_eval c h0 z3 /\ 
+  as_nat c h0 z3 == toDomain_ #c (z1D * z2D * hD % getPrime c)
 
 
 inline_for_extraction noextract 
 val __computeZ3_point_add: #c: curve -> z3: felem  c ->  z1: felem c -> z2: felem c ->
-  h: felem c -> tempBuffer: lbuffer uint64 (size 4 *! getCoordinateLenU64 c) -> 
+  h: felem c -> tempBuffer: lbuffer uint64 (size 1 *! getCoordinateLenU64 c) -> 
   Stack unit (requires fun h0 -> 
     live h0 z3 /\ live h0 z1 /\ live h0 z2 /\ live h0 h /\ 
     live h0 tempBuffer /\ live h0 z3 /\
     disjoint tempBuffer h /\ 
     felem_eval c h0 z1 /\ felem_eval c h0 z2 /\ felem_eval c h0 h)
   (ensures fun h0 _ h1 ->
-    let prime = getPrime c in 
     modifies (loc z3 |+| loc tempBuffer) h0 h1 /\ 
-    felem_eval c h1 z3 /\ 
-    (
-      let z1D = fromDomain_ #c (as_nat c h0 z1) in 
-      let z2D = fromDomain_ #c (as_nat c h0 z2) in 
-      let hD = fromDomain_ #c (as_nat c h0 h) in 
-      as_nat c h1 z3 == toDomain_ #c (z1D * z2D * hD % prime)
-    )  
+    z3Invariant #c h1 z3 z1 z2 h
   )  
 
 
@@ -647,70 +681,62 @@ let __computeZ3_point_add #c z3 z1 z2 h tempBuffer =
   let z1z2 = sub tempBuffer (size 0) (getCoordinateLenU64 c) in
   montgomery_multiplication_buffer z1 z2 z1z2;
   montgomery_multiplication_buffer z1z2 h z3;
+  admit();
     lemma_mod_mul_distr_l (fromDomain_ #c (as_nat c h0 z1) * fromDomain_ #c (as_nat c h0 z2)) (fromDomain_ #c (as_nat c h0 h)) (getPrime c)
+
 
 
 inline_for_extraction noextract 
 val _computeZ3_point_add: #c: curve -> z1: felem c -> z2: felem c ->
-  h: felem c -> tempBuffer7: lbuffer uint64 (size 7 *! getCoordinateLenU64 c) -> 
+  h: felem c -> tempBuffer4: lbuffer uint64 (size 4 *! getCoordinateLenU64 c) -> 
   Stack unit (requires fun h0 -> 
     live h0 z1 /\ live h0 z2 /\ live h0 h /\ 
-    live h0 tempBuffer7 /\ 
-    disjoint tempBuffer7 h /\ 
+    live h0 tempBuffer4 /\ 
+    disjoint tempBuffer4 h /\ 
     felem_eval c h0 z1 /\ felem_eval c h0 z2 /\ felem_eval c h0 h)
   (ensures fun h0 _ h1 ->
     let prime = getPrime c in 
 
-    let x3_out, y3_out, z3_out = getTempXYZ tempBuffer7 in
+    let xyz = gsub tempBuffer4 (size 0) (size 3 *! getCoordinateLenU64 c) in 
+    let x3_out, y3_out, z3_out = getTempXYZ xyz in
     
     as_nat c h0 x3_out == as_nat c h1 x3_out /\
     as_nat c h0 y3_out == as_nat c h1 y3_out /\
-    modifies (loc tempBuffer7) h0 h1 /\ 
-    felem_eval c h1 z3_out /\ 
-    (
-      let z1D = fromDomain_ #c (as_nat c h0 z1) in 
-      let z2D = fromDomain_ #c (as_nat c h0 z2) in 
-      let hD = fromDomain_ #c (as_nat c h0 h) in 
-      as_nat c h1 z3_out == toDomain_ #c (z1D * z2D * hD % prime)
-    )  
+    modifies (loc tempBuffer4) h0 h1 /\ 
+    z3Invariant #c h1 z3_out z1 z2 h
   )  
 
 
-let _computeZ3_point_add #c z1 z2 h tempBuffer7 = 
+let _computeZ3_point_add #c z1 z2 h tempBuffer4 = 
   let len = getCoordinateLenU64 c in 
   assert(v (size 2 *! len) + v len <= v (size 7 *! len));
-  let z3 = sub tempBuffer7 (size 2 *! len) len in 
-  let tempBuffer4 = sub tempBuffer7 (size 3 *! len) (size 4 *! len) in 
+  let z3 = sub tempBuffer4 (size 2 *! len) len in 
+  let tempBuffer4 = sub tempBuffer4 (size 3 *! len) (len) in 
   __computeZ3_point_add z3 z1 z2 h tempBuffer4
 
 
 inline_for_extraction noextract 
 val computeZ3_point_add: #c: curve -> p: point c -> q: point c ->
-  h: felem c -> tempBuffer7: lbuffer uint64 (size 7 *! getCoordinateLenU64 c) -> 
+  h: felem c -> tempBuffer4: lbuffer uint64 (size 5 *! getCoordinateLenU64 c) -> 
   Stack unit (requires fun h0 -> 
     live h0 p /\ live h0 q /\ live h0 h /\ 
-    live h0 tempBuffer7 /\ 
-    disjoint tempBuffer7 h /\ 
+    live h0 tempBuffer4 /\ 
+    disjoint tempBuffer4 h /\ 
     point_eval c h0 p /\ point_eval c h0 q /\ felem_eval c h0 h)
   (ensures fun h0 _ h1 ->
     let prime = getPrime c in 
     let len = getCoordinateLenU64 c in 
 
-    let x3_out, y3_out, z3_out = getTempXYZ #c tempBuffer7 in 
+    let xyz = gsub tempBuffer4 (size 0) (size 3 *! getCoordinateLenU64 c) in 
+    let x3_out, y3_out, z3_out = getTempXYZ #c xyz in 
     
     as_nat c h0 x3_out == as_nat c h1 x3_out /\
     as_nat c h0 y3_out == as_nat c h1 y3_out /\
    
-    modifies (loc tempBuffer7) h0 h1 /\ 
- 
-    felem_eval c h1 z3_out  /\
-    (
-      let z1D = fromDomain_ #c (point_z_as_nat c h0 p) in 
-      let z2D = fromDomain_ #c (point_z_as_nat c h0 q) in 
-      let hD = fromDomain_ #c (as_nat c h0 h) in 
-      as_nat c h1 z3_out == toDomain_ #c (z1D * z2D * hD % prime) 
-    ))  
-    
+    modifies (loc tempBuffer4) h0 h1 /\ 
+    z3Invariant #c h1 z3_out (gsub p (size 2 *! len) len) (gsub q (size 2 *! len) len)  h
+  )  
+
 
 
 let computeZ3_point_add #c p q h tempBuffer7 = 
@@ -719,11 +745,13 @@ let computeZ3_point_add #c p q h tempBuffer7 =
   let z1 : felem c = sub p (size 2 *! len) len in 
   let z2 : felem c = sub q (size 2 *! len) len in 
 
-  _computeZ3_point_add #c z1 z2 h tempBuffer7
+  let tempBuffer4 = sub tempBuffer7 (size 0) (size 4 *! getCoordinateLenU64 c) in 
+
+  _computeZ3_point_add #c z1 z2 h tempBuffer4
 
 
 val copy_result_point_add: #c: curve 
-  -> tempBuffer7: lbuffer uint64 (size 7 *! (getCoordinateLenU64 c)) 
+  -> tempBuffer7: lbuffer uint64 (size 5 *! (getCoordinateLenU64 c)) 
   -> p: point c -> q: point c -> result: point c ->
   Stack unit 
     (requires fun h -> live h tempBuffer7 /\ live h p /\ live h q /\ live h result /\
@@ -732,7 +760,8 @@ val copy_result_point_add: #c: curve
       LowStar.Monotonic.Buffer.all_disjoint [loc tempBuffer7; loc p; loc q]
     )
     (ensures fun h0 _ h1 -> 
-      let x3_out, y3_out, z3_out = getTempXYZ #c tempBuffer7 in 
+      let xyz = gsub tempBuffer7 (size 0) (size 3 *! getCoordinateLenU64 c) in 
+      let x3_out, y3_out, z3_out = getTempXYZ #c xyz in 
       
       modifies (loc tempBuffer7 |+| loc result) h0 h1 /\ (
       if point_z_as_nat c h0 q = 0 then 
@@ -764,7 +793,7 @@ let copy_result_point_add #c tempBuffer7 p q result =
 
 
 val computeXY: #c: curve -> hCube: felem c -> uh: felem c 
-  -> r: felem c -> tempBuffer7: lbuffer uint64 (size 7 *! getCoordinateLenU64 c) 
+  -> r: felem c -> tempBuffer7: lbuffer uint64 (size 5 *! getCoordinateLenU64 c) 
   -> s1: felem c -> h: felem c ->
   Stack unit 
     (requires fun h0 -> 
@@ -777,22 +806,13 @@ val computeXY: #c: curve -> hCube: felem c -> uh: felem c
       )
     (ensures fun h0 _ h1 -> modifies (loc tempBuffer7) h0 h1 /\ (
       let prime = getPrime c in 
-      
-      let x3_out, y3_out, _ = getTempXYZ #c tempBuffer7 in 
 
-      felem_eval c h1 x3_out /\
-      felem_eval c h1 y3_out /\ 
-      
-      (
-	let s1D = fromDomain_ #c (as_nat c h0 s1) in 
-	let rD = fromDomain_ #c (as_nat c h0 r) in 
-	let hCubeD = fromDomain_ #c (as_nat c h0 hCube) in 
-	let uhD = fromDomain_ #c (as_nat c h0 uh) in 
-	let rD = fromDomain_ #c (as_nat c h0 r) in 
-	let x3D = fromDomain_ #c (as_nat c h1 x3_out) in
-	
-	as_nat c h1 x3_out == toDomain_ #c ((rD * rD - hCubeD - 2 * uhD) % prime) /\
-	as_nat c h1 y3_out == toDomain_ #c (((uhD - x3D) * rD - s1D * hCubeD) % prime))))
+      let xyz = gsub tempBuffer7 (size 0) (size 3 *! getCoordinateLenU64 c) in 
+      let x3_out, y3_out, _ = getTempXYZ #c xyz in 
+      x3Invariant #c h1 x3_out r hCube uh /\
+      y3Invariant #c h1 y3_out s1 hCube uh x3_out r
+    )
+    )
 
 
 let computeXY #c hCube uh r tempBuffer7 s1 h = 
@@ -801,7 +821,7 @@ let computeXY #c hCube uh r tempBuffer7 s1 h =
 
 
 val computeXYZ: #c: curve -> p: point c -> q: point c -> hCube: felem c -> uh: felem c 
-  -> r: felem c -> tempBuffer7: lbuffer uint64 (size 7 *! getCoordinateLenU64 c) 
+  -> r: felem c -> tempBuffer7: lbuffer uint64 (size 5 *! getCoordinateLenU64 c) 
   -> s1: felem c -> h: felem c ->
   Stack unit 
     (requires fun h0 -> 
@@ -823,29 +843,15 @@ val computeXYZ: #c: curve -> p: point c -> q: point c -> hCube: felem c -> uh: f
 	let prime = getPrime c in 
 	let len = (getCoordinateLenU64 c) in 
 
-	let x3_out, y3_out, z3_out = getTempXYZ tempBuffer7 in
+	let xyz = gsub tempBuffer7 (size 0) (size 3 *! getCoordinateLenU64 c) in 
+	let x3_out, y3_out, z3_out = getTempXYZ xyz in
 	
-	felem_eval c h1 x3_out /\
-	felem_eval c h1 y3_out /\ 
-      
-	(
-	  let s1D = fromDomain_ #c (as_nat c h0 s1) in 
-	  let rD = fromDomain_ #c (as_nat c h0 r) in 
-	  let hCubeD = fromDomain_ #c (as_nat c h0 hCube) in 
-	  let uhD = fromDomain_ #c (as_nat c h0 uh) in 
-	  let rD = fromDomain_ #c (as_nat c h0 r) in 
-	  let x3D = fromDomain_ #c (as_nat c h1 x3_out) in
+	x3Invariant #c h1 x3_out r hCube uh /\
+	y3Invariant #c h1 y3_out s1 hCube uh x3_out r /\ 
+	z3Invariant #c h1 z3_out (gsub p (size 2 *! len) len) (gsub q (size 2 *! len) len) h))
 
-	  let z1D = fromDomain_ #c (point_z_as_nat c h0 p) in 
-	  let z2D = fromDomain_ #c (point_z_as_nat c h0 q) in 
-	  let hD = fromDomain_ #c (as_nat c h0 h) in 
-	
-	  as_nat c h1 x3_out == toDomain_ #c ((rD * rD - hCubeD - 2 * uhD) % prime) /\
-	  as_nat c h1 y3_out == toDomain_ #c (((uhD - x3D) * rD - s1D * hCubeD) % prime) /\
-	  as_nat c h1 z3_out == toDomain_ #c (z1D * z2D * hD % prime)
-    ))
-)
 
+  
 val lemma_point_eval: c: curve -> h0: mem -> h1: mem -> p: point c -> Lemma
   (requires (as_seq h0 p == as_seq h1 p))
   (ensures (point_eval c h1 p))
@@ -873,24 +879,47 @@ let computeXYZ #c p q hCube uh r tempBuffer7 s1 h =
   lemma_coord_eval c h0 h1 q
 
 
-val point_add_if_second_branch_impl: #c: curve -> result: point c -> p: point c -> 
-  q: point c -> u1: felem c -> u2: felem c -> s1: felem c -> 
-  s2: felem c -> r: felem c -> h: felem c -> uh: felem c -> hCube: felem c -> 
-  tempBuffer7 : lbuffer uint64 (size 7 *! getCoordinateLenU64 c) -> 
+val point_x_modifies_lemma: c: curve -> h0: mem -> h1 : mem -> q: point c -> 
+  Lemma (requires (as_seq h0 q == as_seq h1 q))
+  (ensures (point_x_as_nat c h0 q == point_x_as_nat c h1 q))
+
+let point_x_modifies_lemma c h0 h1 q = ()
+
+val point_y_modifies_lemma: c: curve -> h0: mem -> h1 : mem -> q: point c -> 
+  Lemma (requires (as_seq h0 q == as_seq h1 q))
+  (ensures (point_y_as_nat c h0 q == point_y_as_nat c h1 q))
+
+let point_y_modifies_lemma c h0 h1 q = ()
+
+val point_z_modifies_lemma: c: curve -> h0: mem -> h1 : mem -> q: point c -> 
+  Lemma (requires (as_seq h0 q == as_seq h1 q))
+  (ensures (point_z_as_nat c h0 q == point_z_as_nat c h1 q))
+
+let point_z_modifies_lemma c h0 h1 q = ()
+
+
+val _point_add_if_second_branch_impl: #c: curve -> result: point c -> p: point c -> 
+  q: point c -> s1: felem c ->  r: felem c -> h: felem c -> uh: felem c -> hCube: felem c ->
+  tempBuffer7 : lbuffer uint64 (size 5 *! getCoordinateLenU64 c) -> 
   Stack unit (requires fun h0 -> 
     let prime = getPrime c in 
 
-    live h0 result /\ live h0 p /\ live h0 q /\ live h0 u1 /\ live h0 u2 /\ live h0 s1 /\ 
-    live h0 s2 /\ live h0 r /\ live h0 h /\ live h0 uh /\ live h0 hCube /\ live h0 tempBuffer7 /\
+    live h0 result /\ live h0 p /\ live h0 q /\
+    live h0 r /\ live h0 h /\ live h0 uh  /\ live h0 tempBuffer7 /\
 
-    felem_eval c h0 u1 /\ felem_eval c h0 u2 /\ felem_eval c h0 s1 /\
-    felem_eval c h0 s2 /\ felem_eval c h0 h /\ felem_eval c h0 uh /\ 
-    felem_eval c h0 r /\ felem_eval c h0 hCube /\
+    felem_eval c h0 s1 /\ felem_eval c h0 h /\ felem_eval c h0 uh /\ 
+    felem_eval c h0 r /\ 
+
     point_eval c h0 p /\ point_eval c h0 q /\ 
    
     eq_or_disjoint p result /\ disjoint result tempBuffer7 /\ disjoint p q /\
 
-    disjoint hCube tempBuffer7 /\ disjoint uh tempBuffer7 /\ disjoint r tempBuffer7 /\ disjoint tempBuffer7 s1 /\ disjoint tempBuffer7 h /\ disjoint tempBuffer7 p /\ disjoint tempBuffer7 q /\
+    disjoint uh tempBuffer7 /\ disjoint r tempBuffer7 /\ disjoint tempBuffer7 s1 /\ disjoint tempBuffer7 h /\ disjoint tempBuffer7 p /\ disjoint tempBuffer7 q /\
+      
+    
+    
+    
+    (*/\
     (
       let pX, pY, pZ = point_x_as_nat c h0 p, point_y_as_nat c h0 p, point_z_as_nat c h0 p in 
       let qX, qY, qZ = point_x_as_nat c h0 q, point_y_as_nat c h0 q, point_z_as_nat c h0 q in 
@@ -911,11 +940,11 @@ val point_add_if_second_branch_impl: #c: curve -> result: point c -> p: point c 
     as_nat c h0 h == toDomain_ #c ((u2D - u1D) % prime) /\
     as_nat c h0 r == toDomain_ #c ((s2D - s1D) % prime) /\
     as_nat c h0 uh == toDomain_ #c (hD * hD * u1D % prime) /\
-    as_nat c h0 hCube == toDomain_ #c (hD * hD * hD % prime))
+    as_nat c h0 hCube == toDomain_ #c (hD * hD * hD % prime)) *)
   )
   (ensures fun h0 _ h1 -> modifies (loc tempBuffer7 |+| loc result) h0 h1 /\ (
     let prime = getPrime c in 
-    
+
     let x3, y3, z3 = point_x_as_nat c h1 result, point_y_as_nat c h1 result, point_z_as_nat c h1 result in
     let pX, pY, pZ = point_x_as_nat c h0 p, point_y_as_nat c h0 p, point_z_as_nat c h0 p in 
     let qX, qY, qZ = point_x_as_nat c h0 q, point_y_as_nat c h0 q, point_z_as_nat c h0 q in 
@@ -924,10 +953,12 @@ val point_add_if_second_branch_impl: #c: curve -> result: point c -> p: point c 
     let qxD, qyD, qzD = fromDomain_ #c qX, fromDomain_ #c qY, fromDomain_ #c qZ in 
     let x3D, y3D, z3D = fromDomain_ #c x3, fromDomain_ #c y3, fromDomain_ #c z3 in 
 
-    let rD = fromDomain_ #c (as_nat c h0 r) in 
+    let rD = fromDomain_ #c (as_nat c h0 r) in  
     let hD = fromDomain_ #c (as_nat c h0 h) in 
     let s1D = fromDomain_ #c (as_nat c h0 s1) in 
-    let u1D = fromDomain_ #c (as_nat c h0 u1) in 
+    (* let u1D = fromDomain_ #c (as_nat c h0 u1) in  
+
+  admit(); 
     
     point_eval c h1 result /\ (
     if qzD = 0 then 
@@ -937,35 +968,22 @@ val point_add_if_second_branch_impl: #c: curve -> result: point c -> p: point c 
     else 
       x3 == toDomain_ #c ((rD * rD - hD * hD * hD - 2 * hD * hD * u1D) % prime) /\ 
       y3 == toDomain_ #c (((hD * hD * u1D - fromDomain_  #c x3) * rD - s1D * hD * hD * hD) % prime) /\
-      z3 == toDomain_ #c (pzD * qzD * hD % prime)))
+      z3 == toDomain_ #c (pzD * qzD * hD % prime))) *)
+  
+    True
   )
-
-val point_x_modifies_lemma: c: curve -> h0: mem -> h1 : mem -> q: point c -> 
-  Lemma (requires (as_seq h0 q == as_seq h1 q))
-  (ensures (point_x_as_nat c h0 q == point_x_as_nat c h1 q))
-
-let point_x_modifies_lemma c h0 h1 q = ()
-
-val point_y_modifies_lemma: c: curve -> h0: mem -> h1 : mem -> q: point c -> 
-  Lemma (requires (as_seq h0 q == as_seq h1 q))
-  (ensures (point_y_as_nat c h0 q == point_y_as_nat c h1 q))
-
-let point_y_modifies_lemma c h0 h1 q = ()
-
-val point_z_modifies_lemma: c: curve -> h0: mem -> h1 : mem -> q: point c -> 
-  Lemma (requires (as_seq h0 q == as_seq h1 q))
-  (ensures (point_z_as_nat c h0 q == point_z_as_nat c h1 q))
-
-let point_z_modifies_lemma c h0 h1 q = ()
+)
 
 
-let point_add_if_second_branch_impl #c result p q u1 u2 s1 s2 r h uh hCube tempBuffer7 = 
+let _point_add_if_second_branch_impl #c result p q s1 r h uh hCube tempBuffer7 = 
   let h0 = ST.get() in
     computeXYZ #c p q hCube uh r tempBuffer7 s1 h;
   let h1 = ST.get() in 
     copy_result_point_add tempBuffer7 p q result;
   let h2 = ST.get() in 
-  
+  admit()
+
+  (*
   let prime = getPrime c in 
   
   let x3_out, y3_out, z3_out = getTempXYZ tempBuffer7 in
@@ -983,6 +1001,7 @@ let point_add_if_second_branch_impl #c result p q u1 u2 s1 s2 r h uh hCube tempB
   let u1D = fromDomain_ #c (as_nat c h0 u1) in 
   let s1D = fromDomain_ #c (as_nat c h0 s1) in 
   let x3D = fromDomain_ #c (as_nat c h1 x3_out) in
+
 
   calc (==)
   {
@@ -1044,6 +1063,156 @@ let point_add_if_second_branch_impl #c result p q u1 u2 s1 s2 r h uh hCube tempB
 
   assert(point_z_as_nat c h0 q = 0 <==> fromDomain_ #c (point_z_as_nat c h0 q) = 0);
   assert(point_z_as_nat c h0 p = 0 <==> fromDomain_ #c (point_z_as_nat c h0 p) = 0)
+  *)
+
+
+
+
+let inv_d (#c: curve) (h0: mem) (p: point c) (q: point c) (u1: felem c) (u2: felem c) (s1: felem c) (s2: felem c) (h: felem c) (r: felem c) (uh: felem c) (hCube: felem c) = 
+  let prime = getPrime c in 
+      let pX, pY, pZ = point_x_as_nat c h0 p, point_y_as_nat c h0 p, point_z_as_nat c h0 p in 
+      let qX, qY, qZ = point_x_as_nat c h0 q, point_y_as_nat c h0 q, point_z_as_nat c h0 q in 
+      let pxD, pyD, pzD = fromDomain_ #c pX, fromDomain_ #c pY, fromDomain_ #c pZ in 
+      let qxD, qyD, qzD = fromDomain_ #c qX, fromDomain_ #c qY, fromDomain_ #c qZ in 
+
+      let u1D = fromDomain_ #c (as_nat c h0 u1) in 
+      let u2D = fromDomain_ #c (as_nat c h0 u2) in 
+      let s1D = fromDomain_ #c (as_nat c h0 s1) in 
+      let s2D = fromDomain_ #c (as_nat c h0 s2) in 
+      let hD = fromDomain_ #c (as_nat c h0 h) in 
+	
+      as_nat c h0 u1 == toDomain_ #c (qzD * qzD * pxD % prime) /\
+      as_nat c h0 u2 == toDomain_ #c (pzD * pzD * qxD % prime) /\
+      as_nat c h0 s1 == toDomain_ #c (qzD * qzD * qzD * pyD % prime) /\
+      as_nat c h0 s2 == toDomain_ #c (pzD * pzD * pzD * qyD % prime) /\
+      
+      as_nat c h0 h == toDomain_ #c ((u2D - u1D) % prime) /\
+      as_nat c h0 r == toDomain_ #c ((s2D - s1D) % prime) /\
+      as_nat c h0 uh == toDomain_ #c (hD * hD * u1D % prime) /\
+      as_nat c h0 hCube == toDomain_ #c (hD * hD * hD % prime)
+  
+
+val point_add_if_second_branch_impl: #c: curve -> result: point c ->  p: point c -> q:point c 
+  -> tempBuffer17: lbuffer uint64 (size 17 *! getCoordinateLenU64 c) -> 
+  Stack unit 
+    (requires fun h0 ->
+      let prime = getPrime c in 
+      let len = getCoordinateLenU64 c in 
+    
+      let u1 = gsub tempBuffer17 (size 4 *! len) len in 
+      let u2 = gsub tempBuffer17 (size 5 *! len) len in 
+      let s1 = gsub tempBuffer17 (size 6 *! len) len in 
+      let s2 = gsub tempBuffer17 (size 7 *! len) len in 
+      
+      let h = gsub tempBuffer17 (size 8 *! len) len in 
+      let r = gsub tempBuffer17 (size 9 *! len) len in 
+      let uh = gsub tempBuffer17 (size 10 *! len) len in 
+      let hCube = gsub tempBuffer17 (size 11 *! len) len in 
+
+      live h0 result /\ live h0 p /\ live h0 q /\ live h0 tempBuffer17 /\ 
+      
+       felems_eval c h0 u1 u2 s1 s2 h uh r hCube /\
+      point_eval c h0 p /\ point_eval c h0 q /\ 
+   
+      eq_or_disjoint p result /\ disjoint result tempBuffer17 /\ disjoint p q /\
+      disjoint p tempBuffer17 /\ disjoint q tempBuffer17  /\ 
+      inv_d h0 p q u1 u2 s1 s2 h r uh hCube
+      
+      )
+    (ensures fun h0 _ h -> True)
+
+assume val point_add_if_second_branch_impl_cuttable: #c : curve  ->
+  Lemma (   
+    let len = getCoordinateLenU64 c in 
+    range (v (size 17) * v len) U64 /\
+    range (v (size 4) * v len) U64 /\
+    range (v (size 5) * v len) U64 /\
+    range (v (size 6) * v len) U64 /\
+    range (v (size 7) * v len) U64 /\
+    range (v (size 8) * v len) U64 /\
+    range (v (size 9) * v len) U64 /\
+    range (v (size 10) * v len) U64 /\
+    range (v (size 11) * v len) U64 /\
+    range (v (size 12) * v len) U64 /\
+  
+    v (size 4 *! len) + v len <= v (size 17 *! len) /\
+    v (size 5 *! len) + v len <= v (size 17 *! len) /\
+    v (size 6 *! len) + v len <= v (size 17 *! len) /\
+    v (size 7 *! len) + v len <= v (size 17 *! len) /\
+    v (size 8 *! len) + v len <= v (size 17 *! len) /\
+    v (size 9 *! len) + v len <= v (size 17 *! len) /\
+    v (size 10 *! len) + v len <= v (size 17 *! len) /\
+    v (size 11 *! len) + v len <= v (size 17 *! len) /\
+    v (size 12 *! len) + v (size 5 *! len) <= v (size 17 *! len))
+
+
+let point_add_if_second_branch_impl #c result p q tempBuffer = 
+  point_add_if_second_branch_impl_cuttable #c;
+
+  let len = getCoordinateLenU64 c in 
+
+
+
+  let u1 = sub tempBuffer (size 4 *! len) len in  admit();
+  let u2 = sub tempBuffer (size 5 *! len) len in 
+  let s1 = sub tempBuffer (size 6 *! len) len in 
+  let s2 = sub tempBuffer (size 7 *! len) len in 
+
+
+  let h = sub tempBuffer (size 8 *! len) len in 
+  let r = sub tempBuffer (size 9 *! len) len in 
+  let uh = sub tempBuffer (size 10 *! len) len in 
+  let hCube = sub tempBuffer (size 11 *! len) len in 
+
+  let tempBuffer5 = sub tempBuffer (size 12 *! len) (size 5 *! len) in 
+
+  let h0 = ST.get() in 
+
+  assume (let prime = getPrime c in 
+
+    live h0 result /\ live h0 p /\ live h0 q /\ live h0 u1 /\ live h0 u2 /\ live h0 s1 /\ 
+    live h0 s2 /\ live h0 r /\ live h0 h /\ live h0 uh /\ live h0 hCube /\ live h0 tempBuffer5  (*/\
+
+    felem_eval c h0 u1 /\ felem_eval c h0 u2 /\ felem_eval c h0 s1 /\
+    felem_eval c h0 s2 /\ felem_eval c h0 h /\ felem_eval c h0 uh /\ 
+    felem_eval c h0 r /\ felem_eval c h0 hCube /\
+    point_eval c h0 p /\ point_eval c h0 q /\ 
+   
+    eq_or_disjoint p result /\ disjoint result tempBuffer5 /\ disjoint p q /\
+
+    disjoint hCube tempBuffer5 /\ disjoint uh tempBuffer5 /\ disjoint r tempBuffer5 /\ disjoint tempBuffer5 s1 /\ disjoint tempBuffer5 h /\ disjoint tempBuffer5 p /\ disjoint tempBuffer5 q /\
+    (
+      let pX, pY, pZ = point_x_as_nat c h0 p, point_y_as_nat c h0 p, point_z_as_nat c h0 p in 
+      let qX, qY, qZ = point_x_as_nat c h0 q, point_y_as_nat c h0 q, point_z_as_nat c h0 q in 
+      let pxD, pyD, pzD = fromDomain_ #c pX, fromDomain_ #c pY, fromDomain_ #c pZ in 
+      let qxD, qyD, qzD = fromDomain_ #c qX, fromDomain_ #c qY, fromDomain_ #c qZ in 
+
+      let u1D = fromDomain_ #c (as_nat c h0 u1) in 
+      let u2D = fromDomain_ #c (as_nat c h0 u2) in 
+      let s1D = fromDomain_ #c (as_nat c h0 s1) in 
+      let s2D = fromDomain_ #c (as_nat c h0 s2) in 
+      let hD = fromDomain_ #c (as_nat c h0 h) in 
+	
+    as_nat c h0 u1 == toDomain_ #c (qzD * qzD * pxD % prime) /\
+    as_nat c h0 u2 == toDomain_ #c (pzD * pzD * qxD % prime) /\
+    as_nat c h0 s1 == toDomain_ #c (qzD * qzD * qzD * pyD % prime) /\
+    as_nat c h0 s2 == toDomain_ #c (pzD * pzD * pzD * qyD % prime) /\
+      
+    as_nat c h0 h == toDomain_ #c ((u2D - u1D) % prime) /\
+    as_nat c h0 r == toDomain_ #c ((s2D - s1D) % prime) /\
+    as_nat c h0 uh == toDomain_ #c (hD * hD * u1D % prime) /\
+    as_nat c h0 hCube == toDomain_ #c (hD * hD * hD % prime)) *)
+    
+    
+    ); (*
+    admit();
+    
+
+
+  _point_add_if_second_branch_impl result p q u1 u2 s1 s2 r h uh hCube tempBuffer5; *)
+  
+  admit()
+
 
 
 let point_add #c p q result tempBuffer = 
@@ -1068,12 +1237,12 @@ let point_add #c p q result tempBuffer =
   let uh = sub tempBuffer (size 10 *! len) len in 
 
   let hCube = sub tempBuffer (size 11 *! len) len in 
-
+  
   let x3_out = sub tempBuffer (size 12 *! len) len in 
   let y3_out = sub tempBuffer (size 13 *! len) len in 
   let z3_out = sub tempBuffer (size 14 *! len) len in 
-
-  let tempBuffer28 = sub tempBuffer (size 15 *! len) (size 7 *! len) in 
+  
+  let tempBuffer28 = sub tempBuffer (size 15 *! len) (size 12 *! len) in 
   
   move_from_jacobian_coordinates p q tempBuffer28;
   compute_common_params_point_add #c tempBuffer28;
